Add pattern constr_var functions

extract/DeclExtra.ml
@@ -988,7 +988,7 @@ let constr_in_m (l: lsymbol) (m: mut_adt) : bool =
 
 
 (*TODO: do we need vs?*)
-let rec pat_constr_vars_inner (m: mut_adt) (vs: ty list) (p: pattern) : Svs.t =
+(*let rec pat_constr_vars_inner (m: mut_adt) (vs: ty list) (p: pattern) : Svs.t =
   match p.pat_node with
 | Pwild -> Svs.empty
 | Pvar x -> if vsym_in_m m vs x then Svs.singleton x else Svs.empty
@@ -1012,7 +1012,7 @@ match p.pat_node with
 | Papp (_, _) -> pat_constr_vars_inner m vs p
 | Por (p1, p2) -> Svs.inter (pat_constr_vars m vs p1) (pat_constr_vars m vs p2)
 | Pas (p, y) -> pat_constr_vars m vs p
-| _ -> Svs.empty
+| _ -> Svs.empty*)
 
 let upd_option (hd: vsymbol option) (x: vsymbol) : vsymbol option =
   match hd with
